Kami/Ex/ProcDecSCN.v
@@ -16,10 +16,10 @@ Section ProcDecSCN.
 
   Variables (fetch: AbsFetch addrSize iaddrSize instBytes dataBytes)
             (dec: AbsDec addrSize instBytes dataBytes rfIdx)
-            (exec: AbsExec addrSize iaddrSize instBytes dataBytes rfIdx)
+            (exec: AbsExec addrSize instBytes dataBytes rfIdx)
             (ammio: AbsMMIO addrSize).
 
-  Variable (procInit: ProcInit iaddrSize dataBytes rfIdx)
+  Variable (procInit: ProcInit addrSize dataBytes rfIdx)
            (memInit: MemInit maddrSize).
 
   Definition scmm := scmm Hdb fetch dec exec ammio procInit memInit.
