Kami/Ex/ProcThreeStInl.v
@@ -9,7 +9,7 @@ Section Inlined.
 
   Variables (fetch: AbsFetch addrSize iaddrSize instBytes dataBytes)
             (dec: AbsDec addrSize instBytes dataBytes rfIdx)
-            (exec: AbsExec addrSize iaddrSize instBytes dataBytes rfIdx).
+            (exec: AbsExec addrSize instBytes dataBytes rfIdx).
 
   Variable (d2eElt: Kind).
   Variable (d2ePack:
@@ -21,8 +21,8 @@ Section Inlined.
                 Expr ty (SyntaxKind (Data dataBytes)) -> (* val1 *)
                 Expr ty (SyntaxKind (Data dataBytes)) -> (* val2 *)
                 Expr ty (SyntaxKind (Data instBytes)) -> (* rawInst *)
-                Expr ty (SyntaxKind (Pc iaddrSize)) -> (* curPc *)
-                Expr ty (SyntaxKind (Pc iaddrSize)) -> (* nextPc *)
+                Expr ty (SyntaxKind (Pc addrSize)) -> (* curPc *)
+                Expr ty (SyntaxKind (Pc addrSize)) -> (* nextPc *)
                 Expr ty (SyntaxKind Bool) -> (* epoch *)
                 Expr ty (SyntaxKind d2eElt)).
   Variables
@@ -39,9 +39,9 @@ Section Inlined.
     (d2eRawInst: forall ty, fullType ty (SyntaxKind d2eElt) ->
                             Expr ty (SyntaxKind (Data instBytes)))
     (d2eCurPc: forall ty, fullType ty (SyntaxKind d2eElt) ->
-                          Expr ty (SyntaxKind (Pc iaddrSize)))
+                          Expr ty (SyntaxKind (Pc addrSize)))
     (d2eNextPc: forall ty, fullType ty (SyntaxKind d2eElt) ->
-                           Expr ty (SyntaxKind (Pc iaddrSize)))
+                           Expr ty (SyntaxKind (Pc addrSize)))
     (d2eEpoch: forall ty, fullType ty (SyntaxKind d2eElt) ->
                           Expr ty (SyntaxKind Bool)).
 
@@ -57,7 +57,7 @@ Section Inlined.
     (e2wVal: forall ty, fullType ty (SyntaxKind e2wElt) ->
                         Expr ty (SyntaxKind (Data dataBytes))).
 
-  Variable (init: ProcInit iaddrSize dataBytes rfIdx).
+  Variable (init: ProcInit addrSize dataBytes rfIdx).
 
   Definition p3st := p3st fetch dec exec
                           d2ePack d2eOpType d2eDst d2eAddr d2eByteEn d2eVal1 d2eVal2
